theories/TRAKHTENBROT/Sig2.v
@@ -1,0 +1,134 @@
+(**************************************************************)
+(*   Copyright Dominique Larchey-Wendling [*]                 *)
+(*                                                            *)
+(*                             [*] Affiliation LORIA -- CNRS  *)
+(**************************************************************)
+(*      This file is distributed under the terms of the       *)
+(*         CeCILL v2 FREE SOFTWARE LICENSE AGREEMENT          *)
+(**************************************************************)
+
+Require Import List Arith Bool Lia Eqdep_dec.
+
+From Undecidability.Shared.Libs.DLW.Utils
+  Require Import utils_tac utils_list utils_nat finite.
+
+From Undecidability.Shared.Libs.DLW.Vec 
+  Require Import pos vec.
+
+From Undecidability.Shared.Libs.DLW.Wf 
+  Require Import wf_finite.
+
+From Undecidability.TRAKHTENBROT
+  Require Import notations fol_ops fo_sig fo_terms fo_logic
+                 membership gfp discrete.
+
+Set Implicit Arguments.
+
+Local Notation ø := vec_nil.
+
+Section Σ2_model.
+
+  Variable (X : Type) (M : fo_model (Σrel 2) X).
+
+  Definition Σ2_model_mem a b := fom_rels M tt (a##b##ø).
+
+  Definition Σ2_model_ext := mb_member_ext Σ2_model_mem.
+
+  Infix "≈m" := (mb_equiv Σ2_model_mem) (at level 70).
+
+  Definition Σ2_model_discr := forall a b, a ≈m b <-> a = b.
+
+  Hypothesis ext : Σ2_model_ext.
+
+  (** In a extensional model of Σ2, extentional equivalence is bisimulation *)
+
+  Fact Σ2_model_ext_equiv_bisim a b : a ≈m b -> @fo_bisimilar (Σrel 2) nil (tt::nil) _ M a b.
+  Proof.
+    rewrite <- fom_eq_fol_characterization.
+    revert a b; apply gfp_greatest.
+    + intros R T H1 x y (_ & H2).
+      split; auto.
+      intros ? [].
+    + intros x y Hxy; split.
+      * intros ? [].
+      * intros ? [ <- | [] ] v p. 
+        simpl in *.
+        vec split v with a; vec split v with b; vec nil v; clear v.
+        analyse pos p; simpl.
+        - split; apply ext; auto.
+          intro; symmetry; apply Hxy. 
+        - apply Hxy.
+  Qed.
+
+End Σ2_model.
+
+Section Sig2_extensional.
+
+  (** If a formula A of Σ2 is satisfiable in some finite & decidable
+      and extensional model, it is also satisfiable in a 
+      finite & decidable & extensional model where extensional
+      identity is equality *)
+
+  Variables (X : Type) 
+            (M : fo_model (Σrel 2) X)
+            (Mfin : finite_t X)
+            (Mdec : fo_model_dec M)
+            (Mext : Σ2_model_ext M)
+            (φ : nat -> X) (A : fol_form (Σrel 2)) 
+            (HA : fol_sem M φ A).
+
+    Let mem a b := fom_rels M tt (a##b##ø).
+
+    Infix "∈m" := mem (at level 70).
+    Infix "≈m" := (mb_equiv mem) (at level 70).
+
+    Let discr := @fo_fin_model_discretize (Σrel 2) nil (tt::nil) _ Mfin M Mdec. 
+  
+    Let n := projT1 discr.
+    Let Md : fo_model (Σrel 2) (pos n).
+    Proof. apply (projT1 (projT2 discr)). Defined.
+    Let Mb : fo_model_dec Md.
+    Proof. apply (projT1 (projT2 (projT2 discr))). Qed.
+    Let p : @fo_projection (Σrel 2) nil (tt::nil) _ M _ Md.
+    Proof. apply (projT1 (projT2 (projT2 (projT2 discr)))). Qed.
+    Let H x y : @fo_bisimilar (Σrel 2) nil (tt::nil) _ Md x y <-> x = y.
+    Proof. apply (projT2 (projT2 (projT2 (projT2 discr)))). Qed.
+
+    Let extensional : Σ2_model_ext Md.
+    Proof.
+      revert Mext.
+      unfold Σ2_model_ext, Σ2_model_mem.
+      rewrite <- Σ2_extensional_spec with (ψ := fun n => p (φ n)).
+      rewrite <- Σ2_extensional_spec with (ψ := φ).
+      apply fo_model_projection with (ls := nil) (lr := tt::nil) (p := p); auto.
+      all: intros []; simpl; auto.
+    Qed.
+
+    Let discrete : Σ2_model_discr Md.
+    Proof.
+      intros x y; split.
+      2: intros []; apply mb_equiv_refl.
+      rewrite <- H.
+      apply Σ2_model_ext_equiv_bisim; auto.
+    Qed.
+
+    Theorem Sig2_ext_discr : 
+        { Y : Type & 
+        { K : fo_model (Σrel 2) Y &
+        { _ : finite_t Y &
+        { _ : fo_model_dec K & 
+        { _ : Σ2_model_ext K &
+        { _ : Σ2_model_discr K & 
+        { ψ | fol_sem K ψ A }}}}}}}.
+    Proof.
+      exists (pos n), Md.
+      exists. { apply finite_t_pos. }
+      exists Mb, extensional, discrete.
+      exists (fun n => p (φ n)).
+      revert HA.
+      apply fo_model_projection with (ls := nil) (lr := tt::nil) (p := p); auto.
+      all: intros []; simpl; auto.
+      all: unfold incl; cbn; simpl; try tauto.
+    Qed. 
+
+End Sig2_extensional.
