theories/TRAKHTENBROT/Sig_Sig2.v
@@ -1,0 +1,846 @@
+(**************************************************************)
+(*   Copyright Dominique Larchey-Wendling [*]                 *)
+(*                                                            *)
+(*                             [*] Affiliation LORIA -- CNRS  *)
+(**************************************************************)
+(*      This file is distributed under the terms of the       *)
+(*         CeCILL v2 FREE SOFTWARE LICENSE AGREEMENT          *)
+(**************************************************************)
+
+Require Import List Arith Bool Lia Eqdep_dec.
+
+From Undecidability.Shared.Libs.DLW.Utils
+  Require Import utils_tac utils_list utils_nat finite.
+
+From Undecidability.Shared.Libs.DLW.Vec 
+  Require Import pos vec.
+
+From Undecidability.Shared.Libs.DLW.Wf 
+  Require Import wf_finite.
+
+From Undecidability.TRAKHTENBROT
+  Require Import notations utils fol_ops fo_sig fo_terms fo_logic fo_sat
+                 membership hfs rels_hfs Sig2.
+
+Set Implicit Arguments.
+
+Local Notation ø := vec_nil.
+
+Fact nat_pos_rect (P : nat -> Type) n :
+           (forall p : pos n, P (pos2nat p))
+        -> (forall i, P (i+n))
+        -> forall i, P i.
+Proof.
+  intros H1 H2 i.
+  destruct (le_lt_dec n i) as [ H | H ].
+  + replace i with ((i-n)+n) by lia; apply H2.
+  + rewrite <- (pos2nat_nat2pos H); apply H1.
+Qed.
+
+Section Sig_Sig2_encoding.
+
+  Variable (Σ : fo_signature).
+
+  Notation Σ2 := (Σrel 2).
+
+  Infix "∈" := Σ2_mem.
+  Infix "≈" := Σ2_equiv.
+  Infix "⊆" := Σ2_incl.
+
+  Notation 𝕋 := (fol_term Σ).
+  Notation 𝔽 := (fol_form Σ).
+
+  Notation 𝕋2 := (fol_term Σ2).
+  Notation 𝔽2 := (fol_form Σ2).
+
+  Section removing_symbols_from_terms.
+
+    Variable (ρ : syms Σ -> nat)
+             (µ : rels Σ -> nat)
+             (d : nat).
+
+    Local Fixpoint fot_rem_syms r n (t : 𝕋) : 𝔽2 :=
+      match t with
+        | in_var i   => r ≈ i+n
+        | in_fot s v => let a := ar_syms _ s
+                     in let v1 := vec_set_pos (fun p : pos a 
+                              => fot_rem_syms (pos2nat p) (n+a) (vec_pos v p))
+                     in let v2 := vec_set_pos (fun p : pos a
+                              => pos2nat p ∈ d+n+a)
+                     in let w := vec_set_pos (fun p : pos a => pos2nat p)
+                     in let A := Σ2_is_tuple_in (ρ s+n+a) (r+a##w)
+                     in let B := fol_vec_fa v1
+                     in let C := fol_vec_fa v2
+                     in fol_mquant fol_ex (ar_syms _ s) (A ⟑ B ⟑ C)
+      end.
+
+    Local Fact for_rem_syms r n t i : In i (fol_vars (fot_rem_syms r n t)) 
+                             -> i = r \/ (exists j, i = j+n /\ In j (d::fo_term_vars t))
+                                      \/ (exists s, i = ρ s+n /\ In s (fo_term_syms t)).
+    Proof.
+      revert r n i; induction t as [ j | s v IH ]; intros r n i.
+      + simpl; repeat (intros [ <- | H ]; [ | revert H]); try tauto; right; left; exists j; auto.
+      + simpl fot_rem_syms.
+        rewrite fol_vars_mquant, in_flat_map.
+        intros (x & H1 & H2).
+        rewrite !fol_vars_bin, !in_app_iff, !fol_vars_vec_fa, !in_flat_map in H1.
+        revert H1; intros [ H1 | [ (y & H1 & H3) | (y & H1 & H3) ] ].
+        * apply Σ2_is_tuple_in_vars in H1; simpl in H1.
+          rewrite vec_list_vec_set_pos, in_map_iff in H1.
+          destruct H1 as [ <- | [ <- | (p & <- & Hp) ] ].
+          - destruct (le_lt_dec (ar_syms Σ s) (ρ s + n + ar_syms Σ s)); try lia.
+            destruct H2 as [ <- | [] ].
+            do 2 right; exists s; split; try lia; simpl; auto.
+          - destruct (le_lt_dec (ar_syms Σ s) (r + ar_syms Σ s)); try lia.
+            destruct H2 as [ <- | [] ]; left; lia.
+          - destruct (le_lt_dec (ar_syms Σ s) (pos2nat p)); simpl in H2; try tauto. 
+            generalize (pos2nat_prop p); try lia.
+        * rewrite vec_list_vec_set_pos, in_map_iff in H1.
+          destruct H1 as (p & <- & H1).
+          apply IH in H3.
+          destruct H3 as [ -> | [ (j & -> & H3) | (s' & -> & H3) ] ].
+          - destruct (le_lt_dec (ar_syms Σ s) (pos2nat p)); simpl in H2; try tauto.
+            generalize (pos2nat_prop p); try lia.
+          - destruct (le_lt_dec (ar_syms Σ s) (j + (n + ar_syms Σ s))); try lia.
+            destruct H2 as [ <- | [] ].
+            right; left; exists j; split; try lia. 
+            destruct H3 as [ H3 | H3 ]; try (simpl; auto; fail); right.
+            rew fot; rewrite in_flat_map.
+            exists (vec_pos v p); split; auto.
+            apply in_vec_list, in_vec_pos.
+          - destruct (le_lt_dec (ar_syms Σ s) (ρ s' + (n + ar_syms Σ s))); try lia.
+            destruct H2 as [ <- | [] ].
+            do 2 right; exists s'; split; try lia.
+            rew fot; simpl; rewrite in_flat_map.
+            right; exists (vec_pos v p); split; auto.
+            apply in_vec_list, in_vec_pos.
+        * rewrite vec_list_vec_set_pos, in_map_iff in H1.
+          destruct H1 as (p & <- & H1).
+          simpl in H3.
+          destruct H3 as [ <- | [ <- | [] ] ].
+          - destruct (le_lt_dec (ar_syms Σ s) (pos2nat p)); simpl in H2; try tauto.
+            generalize (pos2nat_prop p); try lia.
+          - destruct (le_lt_dec (ar_syms Σ s) (d + n + ar_syms Σ s)); try lia.
+            destruct H2 as [ <- | [] ].
+            right; left; exists d; split; simpl; auto; lia.
+    Qed.
+
+    Local Definition fol_rem_atom n (s : rels Σ) (vt : vec 𝕋 (ar_rels _ s) ) : 𝔽2 :=
+         let a := ar_rels _ s
+      in let v1 := vec_set_pos (fun p : pos a 
+              => fot_rem_syms (pos2nat p) (n+a) (vec_pos vt p))
+      in let v2 := vec_set_pos (fun p : pos a
+              => pos2nat p ∈ d+n+a)
+      in let w := vec_set_pos (fun p : pos a => pos2nat p)
+      in let A := Σ2_is_tuple_in (µ s+n+a) w
+      in let B := fol_vec_fa v1
+      in let C := fol_vec_fa v2
+      in fol_mquant fol_ex a (A ⟑ B ⟑ C).
+
+    Fact fol_rem_atom_vars n s vt i : In i (fol_vars (fol_rem_atom n s vt))
+                                   ->    (exists j, i = j+n /\ In j (d::flat_map fo_term_vars (vec_list vt)))
+                                      \/ (exists s, i = ρ s+n /\ In s (flat_map fo_term_syms (vec_list vt)))
+                                      \/ i = µ s+n.
+    Proof.
+      unfold fol_rem_atom.
+      rewrite fol_vars_mquant, in_flat_map.
+      intros (x & H1 & H2); revert H1.
+      rewrite !fol_vars_bin, !in_app_iff, !fol_vars_vec_fa, !in_flat_map.
+      intros [ H1 | [ (y & H1 & H3) | (y & H1 & H3) ] ].
+      + apply Σ2_is_tuple_in_vars in H1; simpl in H1.
+        rewrite vec_list_vec_set_pos, in_map_iff in H1.
+        destruct H1 as [ <- | (p & <- & Hp) ].
+        * destruct (le_lt_dec (ar_rels Σ s) (µ s + n + ar_rels Σ s)); try lia.
+          destruct H2 as [ <- | [] ].
+          do 2 right; lia.
+        * destruct (le_lt_dec (ar_rels Σ s) (pos2nat p)); simpl in H2; try tauto. 
+          generalize (pos2nat_prop p); try lia.
+      + rewrite vec_list_vec_set_pos, in_map_iff in H1.
+        destruct H1 as (p & <- & H1).
+        apply for_rem_syms in H3.
+        destruct H3 as [ -> | [ (j & -> & H3) | (s' & -> & H3) ] ].
+        * destruct (le_lt_dec (ar_rels Σ s) (pos2nat p)); simpl in H2; try tauto. 
+          generalize (pos2nat_prop p); try lia.
+        * destruct (le_lt_dec (ar_rels Σ s) (j + (n + ar_rels Σ s))); try lia.
+          destruct H2 as [ <- | [] ].
+          left; exists j; split; try lia.
+          destruct H3 as [ H3 | H3 ]; subst; try (simpl; auto; fail); right.
+          apply in_flat_map.
+          exists (vec_pos vt p); split; auto.
+          apply in_vec_list, in_vec_pos.
+        * destruct (le_lt_dec (ar_rels Σ s) (ρ s' + (n + ar_rels Σ s))); try lia.
+          destruct H2 as [ <- | [] ].
+          right; left; exists s'; split; try lia.
+          apply in_flat_map.
+          exists (vec_pos vt p); split; auto.
+          apply in_vec_list, in_vec_pos.
+      + rewrite vec_list_vec_set_pos, in_map_iff in H1.
+        destruct H1 as (p & <- & H1).
+        simpl in H3.
+        destruct H3 as [ <- | [ <- | [] ] ].
+        - destruct (le_lt_dec (ar_rels Σ s) (pos2nat p)); simpl in H2; try tauto.
+          generalize (pos2nat_prop p); try lia.
+        - destruct (le_lt_dec (ar_rels Σ s) (d + n + ar_rels Σ s)); try lia.
+          destruct H2 as [ <- | [] ].
+          left; exists d; simpl; split; auto; lia.
+    Qed.
+
+    Variable (X : Type) (MX : fo_model Σ X)
+             (Y : Type) (MY : fo_model Σ2 Y) (dy : Y).
+
+    Let mem x y := fom_rels MY tt (x##y##ø).
+
+    Hypothesis (HY1 : mb_member_ext mem)
+               (HY2 : forall u v, mb_equiv mem u v <-> u = v).
+
+    Hypothesis (f : X -> Y) (g : Y -> X) 
+               (Hfg1 : forall x, mem (f x) dy)
+               (Hfg2 : forall y, mem y dy -> exists x, y = f x) 
+               (Hfg3 : forall x, g (f x) = x).
+
+    Let f_equiv u v : u = v <-> f u = f v.
+    Proof.
+      split.
+      + intros []; auto.
+      + intros H; rewrite <- (Hfg3 u), H, Hfg3; auto.
+    Qed.
+
+    Hypothesis (φ : nat -> X).
+
+    Theorem fot_rem_syms_sem t r x ψ n :
+                                   (forall s v x,   In s (fo_term_syms t)
+                                    ->  x = fom_syms MX s v 
+                                   <-> mb_is_tuple_in mem (ψ (ρ s+n)) (f x##vec_map f v))
+                                -> (forall i, In i (fo_term_vars t) -> ψ (i+n) = f (φ i))
+                                -> ψ (d+n) = dy
+                                -> ψ r = f x
+                                -> x = fo_term_sem MX φ t
+                               <-> fol_sem MY ψ (fot_rem_syms r n t).
+    Proof.
+      revert r n ψ x.
+      induction t as [ i | s vt IH ]; intros r n ψ x Hρ H1 H3 H2.
+      + simpl fot_rem_syms.
+        rewrite Σ2_equiv_spec. 
+        unfold mem in HY2. 
+        rewrite HY2; rew fot.
+        rewrite H1, H2. 
+        apply f_equiv.
+        rew fot; simpl; auto.
+      + simpl fot_rem_syms.
+        rewrite fol_sem_mexists.
+        split.
+        * rew fot; intros E.
+          exists (vec_map (fun t => f (fo_term_sem MX φ t)) vt).
+          msplit 2.
+          - rewrite Σ2_is_tuple_in_spec.
+            simpl vec_map; simpl env_vlift.
+            rewrite !env_vlift_fix1.
+            rewrite vec_map_set_pos.
+            match goal with
+              | |- mb_is_tuple_in _ _ (_##?t) => assert (H : t = vec_map f (vec_map (fo_term_sem MX φ) vt))
+            end.
+            { apply vec_pos_ext; intros p; rew vec.
+              rewrite env_vlift_fix0; rew vec. }
+            rewrite H; clear H.
+            rewrite H2.
+            apply Hρ; auto.
+            rew fot; simpl; auto.
+          - rewrite fol_sem_vec_fa; intros p.
+            rew vec; simpl.
+            rewrite <- IH.
+            ++ reflexivity.
+            ++ intros; rewrite plus_assoc, env_vlift_fix1; auto.
+               apply Hρ; rew fot; right; apply in_flat_map.
+               exists (vec_pos vt p); split; auto.
+               apply in_vec_list, in_vec_pos.
+            ++ intros i Hi; rewrite plus_assoc, env_vlift_fix1; auto.
+               apply H1; rew fot; apply in_flat_map.
+               exists (vec_pos vt p); split; auto.
+               apply in_vec_list, in_vec_pos.
+            ++ rewrite plus_assoc, env_vlift_fix1; auto. 
+            ++ rewrite env_vlift_fix0; rew vec.
+          - rewrite fol_sem_vec_fa; intros p; rew vec; simpl.
+            rewrite env_vlift_fix0, env_vlift_fix1; rew vec.
+            rewrite H3; apply Hfg1.
+        * intros (w & H4 & H5 & H6).
+          rewrite Σ2_is_tuple_in_spec in H4; simpl in H4.
+          rewrite !env_vlift_fix1 in H4.
+          rewrite vec_map_set_pos in H4.
+          replace (vec_set_pos (fun p : pos (ar_syms Σ s) => env_vlift ψ w (pos2nat p)))
+            with w in H4.
+          2: apply vec_pos_ext; intro; rew vec; rewrite env_vlift_fix0; auto.
+          rewrite H2 in H4.
+          rewrite fol_sem_vec_fa in H6.
+          assert (H7: forall p, mem (vec_pos w p) dy).
+          { intros p; generalize (H6 p); rew vec; simpl.
+            rewrite env_vlift_fix0, env_vlift_fix1, H3; auto. }
+          clear H6.
+          assert (H8: forall p, exists x, vec_pos w p = f x).
+          { intros; apply Hfg2; auto. }
+          apply vec_reif in H8.
+          destruct H8 as (v' & H8).
+          rewrite fol_sem_vec_fa in H5.
+          assert (H6: forall p, fol_sem MY (env_vlift ψ w) (fot_rem_syms (pos2nat p) (n + ar_syms _ s) (vec_pos vt p))).
+          { intros p; generalize (H5 p); rew vec. }
+          clear H5.
+          assert (H5 : forall p, vec_pos v' p = fo_term_sem MX φ (vec_pos vt p)).
+          { intros p.
+            generalize (H6 p).
+            apply IH; auto.
+            + intros s' v x' H.
+              rewrite plus_assoc, env_vlift_fix1.
+              apply Hρ; rew fot; right; apply in_flat_map.
+              exists (vec_pos vt p); split; auto.
+              apply in_vec_list, in_vec_pos.
+            + intros i Hi; rewrite plus_assoc, env_vlift_fix1; auto.
+              apply H1; rew fot; apply in_flat_map.
+              exists (vec_pos vt p); split; auto.
+              apply in_vec_list, in_vec_pos.
+            + rewrite plus_assoc, env_vlift_fix1; auto.
+            + rewrite env_vlift_fix0; auto. }
+          rew fot.
+          apply Hρ; auto.
+          - rew fot; simpl; auto.
+          - rewrite vec_map_map.
+            revert H4.
+            apply fol_equiv_ext; do 2 f_equal.
+            apply vec_pos_ext; intros p; rew vec.
+            rewrite H8, H5; auto.
+    Qed.
+
+    Hypothesis (ψ : nat -> Y) (s : rels Σ) (vt : vec 𝕋 (ar_rels _ s))
+               (Hρ : forall s' v x,  In s' (flat_map fo_term_syms (vec_list vt))
+                                 -> x = fom_syms MX s' v 
+                                <-> mb_is_tuple_in mem (ψ (ρ s')) (f x##vec_map f v))
+               (Hµ : forall v, fom_rels MX s v 
+                 <-> mb_is_tuple_in mem (ψ (µ s)) (vec_map f v))
+               (H1 : forall i, In i (flat_map fo_term_vars (vec_list vt)) -> ψ i = f (φ i))
+               (H2 : ψ d = dy).
+
+    Theorem fol_rem_atom_sem : fol_sem MX φ (fol_atom s vt)
+                           <-> fol_sem MY ψ (fol_rem_atom 0 s vt).
+    Proof.
+      simpl; rewrite Hµ; auto.
+      unfold fol_rem_atom. 
+      rewrite fol_sem_mexists.
+      split; auto.
+      + intros H.
+        exists (vec_map (fun t => f (fo_term_sem MX φ t)) vt).
+        msplit 2.
+        * rewrite Σ2_is_tuple_in_spec.
+          rewrite env_vlift_fix1.
+          revert H; apply fol_equiv_ext; f_equal.
+          - f_equal; lia.
+          - apply vec_pos_ext; intros p; rew vec.
+            rewrite env_vlift_fix0; rew vec.
+        * rewrite fol_sem_vec_fa; intros p; rew vec.
+          rewrite <- fot_rem_syms_sem.
+          - reflexivity.
+          - intros; rewrite plus_assoc, env_vlift_fix1; auto.
+            rewrite plus_comm; simpl; auto.
+            apply Hρ, in_flat_map.
+            exists (vec_pos vt p); split; auto.
+            apply in_vec_list, in_vec_pos.
+          - intros i Hi; simpl.
+            rewrite env_vlift_fix1; auto.
+            apply H1, in_flat_map.
+            exists (vec_pos vt p); split; auto.
+            apply in_vec_list, in_vec_pos.
+          - simpl; rewrite env_vlift_fix1; auto.
+          - rewrite env_vlift_fix0; rew vec.
+        * rewrite fol_sem_vec_fa; intros p; rew vec.
+          simpl; rewrite env_vlift_fix0, env_vlift_fix1; rew vec.
+          rewrite plus_comm; simpl.
+          rewrite H2; apply Hfg1.
+      + intros (w & H3 & H4 & H5).
+        rewrite Σ2_is_tuple_in_spec in H3; simpl in H3.
+        rewrite  Nat.add_0_r, !env_vlift_fix1 in H3.
+        rewrite vec_map_set_pos in H3.
+        replace (vec_set_pos (fun p : pos (ar_rels _ s) => env_vlift ψ w (pos2nat p)))
+          with w in H3.
+        2: apply vec_pos_ext; intro; rew vec; rewrite env_vlift_fix0; auto.
+        rewrite fol_sem_vec_fa in H5.
+        assert (H7: forall p, mem (vec_pos w p) dy).
+        { intros p; generalize (H5 p); rew vec; simpl.
+          rewrite Nat.add_0_r, env_vlift_fix0, env_vlift_fix1, H2; auto. }
+        clear H5.
+        assert (H8: forall p, exists x, vec_pos w p = f x).
+        { intros; apply Hfg2; auto. }
+        apply vec_reif in H8.
+        destruct H8 as (v' & H8).
+        rewrite fol_sem_vec_fa in H4.
+        assert (H6: forall p, fol_sem MY (env_vlift ψ w) (fot_rem_syms (pos2nat p) (ar_rels _ s) (vec_pos vt p))).
+        { intros p; generalize (H4 p); rew vec. }
+        clear H4.
+        assert (H5 : forall p, vec_pos v' p = fo_term_sem MX φ (vec_pos vt p)).
+        { intros p.
+          generalize (H6 p).
+          apply fot_rem_syms_sem; auto.
+          + intros; rewrite env_vlift_fix1; auto.
+            apply Hρ, in_flat_map.
+            exists (vec_pos vt p); split; auto.
+            apply in_vec_list, in_vec_pos.
+          + intros i Hi; rewrite env_vlift_fix1.
+            apply H1, in_flat_map.
+            exists (vec_pos vt p); split; auto.
+            apply in_vec_list, in_vec_pos. 
+          + rewrite env_vlift_fix1; auto.
+          + rewrite env_vlift_fix0; auto. }
+        rew fot.
+        revert H3.
+        apply fol_equiv_ext; do 2 f_equal.
+        apply vec_pos_ext; intros p; rew vec.
+        rewrite H8, H5; auto.
+    Qed.
+
+  End removing_symbols_from_terms.
+
+  Section all.
+
+    Implicit Types (ρ : syms Σ -> nat)
+                   (µ : rels Σ -> nat)
+                   (d : nat).
+
+    Fixpoint Σ_Σ2 ρ µ d (A : 𝔽) : 𝔽2 :=
+      match A with
+        | ⊥              => ⊥
+        | fol_atom s v   => fol_rem_atom ρ µ d 0 s v 
+        | fol_bin b A B  => fol_bin b (Σ_Σ2 ρ µ d A) (Σ_Σ2 ρ µ d B)
+        | ∀ A            => ∀ 0 ∈ (S d) ⤑ Σ_Σ2 (fun s => S (ρ s)) (fun s => S (µ s)) (S d) A
+        | ∃ A            => ∃ 0 ∈ (S d) ⟑ Σ_Σ2 (fun s => S (ρ s)) (fun s => S (µ s)) (S d) A
+      end.
+
+    Fact Σ_Σ2_vars ρ µ d A : incl (fol_vars (Σ_Σ2 ρ µ d A)) 
+                                  (d::fol_vars A++map ρ (fol_syms A)++map µ (fol_rels A)).
+    Proof.
+      revert ρ µ d; induction A as [ | r v | b A HA B HB | [] A HA ]; intros ρ µ d i Hi.
+      + destruct Hi.
+      + apply fol_rem_atom_vars in Hi.
+        simpl; rewrite !in_app_iff.
+        destruct Hi as [ (j & -> & [ <- | Hj ]) | [ (s' & -> & Hs') | -> ] ]; rewrite <- plus_comm; simpl; auto.
+        right; right; left; apply in_map_iff; exists s'; auto.
+      + simpl in *; rewrite !in_app_iff in *.
+        destruct Hi as [ Hi | Hi ]; [ apply HA in Hi | apply HB in Hi ];
+          simpl in *; rewrite !map_app, !in_app_iff in *; tauto.
+      + simpl in *; rewrite !in_app_iff, !in_flat_map, !in_map_iff in *.
+        destruct Hi as [ Hi | (x & Hi & H2) ]; auto.
+        apply HA in Hi.
+        simpl in *; rewrite !in_app_iff, !in_map_iff in *. 
+        destruct Hi as [ <- | [ Hi | [ (s' & <- & Hi) | (s' & <- & Hi) ] ] ].
+        * simpl in H2; tauto.
+        * right; left; exists x; auto.
+        * destruct H2 as [ <- | [] ]; right; right; left; exists s'; auto.
+        * destruct H2 as [ <- | [] ]; right; right; right; exists s'; auto.
+      + simpl in *; rewrite !in_app_iff, !in_flat_map, !in_map_iff in *.
+        destruct Hi as [ Hi | (x & Hi & H2) ]; auto.
+        apply HA in Hi.
+        simpl in *; rewrite !in_app_iff, !in_map_iff in *. 
+        destruct Hi as [ <- | [ Hi | [ (s' & <- & Hi) | (s' & <- & Hi) ] ] ].
+        * simpl in H2; tauto.
+        * right; left; exists x; auto.
+        * destruct H2 as [ <- | [] ]; right; right; left; exists s'; auto.
+        * destruct H2 as [ <- | [] ]; right; right; right; exists s'; auto.
+    Qed.
+
+    Variable (X : Type) (MX : fo_model Σ X)
+             (Y : Type) (MY : fo_model Σ2 Y) (dy : Y).
+
+    Let mem x y := fom_rels MY tt (x##y##ø).
+
+    Hypothesis (HY1 : mb_member_ext mem)
+               (HY2 : forall u v, mb_equiv mem u v <-> u = v).
+
+    Hypothesis (f : X -> Y) (g : Y -> X) 
+               (Hfg1 : forall x, mem (f x) dy)
+               (Hfg2 : forall y, mem y dy -> exists x, y = f x) 
+               (Hfg3 : forall x, g (f x) = x).
+
+    Let f_equiv u v : u = v <-> f u = f v.
+    Proof.
+      split.
+      + intros []; auto.
+      + intros H; rewrite <- (Hfg3 u), H, Hfg3; auto.
+    Qed.
+
+    Hypothesis (ρ : syms Σ -> nat)
+               (µ : rels Σ -> nat)
+               (d : nat)
+               (φ : nat -> X) (ψ : nat -> Y)
+               (F : 𝔽)
+               (Hφ : forall i, In i (fol_vars F) -> ψ i = f (φ i))
+               (Hψ : ψ d = dy)
+               (Hρ : forall s v x,  In s (fol_syms F)
+                                 -> x = fom_syms MX s v 
+                                <-> mb_is_tuple_in mem (ψ (ρ s)) (f x##vec_map f v))
+               (Hµ : forall s v,    In s (fol_rels F)
+                                 -> fom_rels MX s v 
+                                <-> mb_is_tuple_in mem (ψ (µ s)) (vec_map f v)).
+
+    Theorem Σ_Σ2_sem : fol_sem MX φ F
+                   <-> fol_sem MY ψ (Σ_Σ2 ρ µ d F).
+    Proof.
+      revert ρ µ d φ ψ Hρ Hµ Hφ Hψ.
+      induction F as [ | r vt | b A HA B HB | [] A HA ]; intros ρ µ d φ ψ Hρ Hµ H1 H2.
+      + simpl; tauto.
+      + apply fol_rem_atom_sem with (dy := dy) (4 := Hfg3); auto.
+        intros; apply Hµ; simpl; auto.
+      + simpl Σ_Σ2; rewrite !fol_sem_bin_fix.
+        apply fol_bin_sem_ext; [ apply HA | apply HB ]; auto; intros; 
+          (apply Hρ || apply Hµ || apply H1 ); apply in_app_iff; auto.
+      + simpl; split.
+        * intros (x & Hx).
+          exists (f x); split.
+          - rewrite H2; apply Hfg1.
+          - revert Hx; apply HA; auto.
+            intros [] ?; simpl; auto.
+            apply H1, in_flat_map.
+            exists (S n); simpl; auto.
+        * intros (y & H3 & H4).
+          destruct (Hfg2 y) as (x & Hx).
+          - rewrite <- H2; auto.
+          - exists x.
+            revert H4; apply HA; auto.
+            intros [] ?; simpl; auto.
+            apply H1, in_flat_map.
+            exists (S n); simpl; auto.
+      + simpl; split.
+        * intros H y Hy.
+          rewrite H2 in Hy.
+          destruct (Hfg2 _ Hy) as (x & Hx).
+          generalize (H x); apply HA; auto.
+          intros [] ?; simpl; auto.
+          apply H1, in_flat_map.
+          exists (S n); simpl; auto.
+        * intros H x.
+          specialize (H (f x)).
+          rewrite H2 in H.
+          generalize (H (Hfg1 _)); apply HA; auto.
+          intros [] ?; simpl; auto.
+          apply H1, in_flat_map.
+          exists (S n); simpl; auto.
+    Qed.
+
+  End all.
+
+  Hypothesis (Hs : discrete (syms Σ))
+             (Hr : discrete (rels Σ)).
+
+  Check Σ_Σ2.
+  Check Σ_Σ2_sem.
+  Check Σ_Σ2_vars.
+
+  Variable A : fol_form Σ.
+
+  Let Ds := list_discrete_bij_nat (fol_syms A) Hs.
+  Let Dr := list_discrete_bij_nat (fol_rels A) Hr.
+
+  Let x0 := 0.
+  Let d  := 1.
+
+  Let ns  := projT1 Ds.
+  Let ρ s := 2 + projT1 (projT2 Ds) s.
+
+  Let nr  := projT1 Dr.
+  Let µ r := 2 + ns + projT1 (projT2 Dr) r.
+
+  Let B := fol_subst (fun i => £ (i+2+ns+nr)) A.
+
+  Definition Σ_Σ2_enc := 
+                Σ2_extensional 
+              ⟑ x0 ∈ d
+              ⟑ Σ2_transitive d
+              ⟑ Σ2_list_in d (fol_vars B) 
+              ⟑ fol_lconj (map (fun s => Σ2_is_fun d (ρ s) ⟑ Σ2_is_tot (ar_syms _ s) d (ρ s)) (fol_syms A))
+              ⟑ Σ_Σ2 ρ µ d B.
+
+  Section SAT2_SAT.
+
+    Variables (Y : Type) 
+              (M2 : fo_model (Σrel 2) Y)
+              (M2fin : finite_t Y)
+              (M2dec : fo_model_dec M2)
+              (ψ : nat -> Y)
+              (HA : fol_sem M2 ψ Σ_Σ2_enc).
+
+    Let mem a b := fom_rels M2 tt (a##b##ø).
+
+    Infix "∈m" := mem (at level 70).
+    Infix "≈m" := (mb_equiv mem) (at level 70).
+
+    Hypothesis Mmem : forall x y, x ≈m y <-> x = y.
+
+    Let mem_dec : forall x y, { x ∈m y } + { ~ x ∈m y }.
+    Proof. intros x y; apply (@M2dec tt). Qed.
+
+    Let equiv_refl x : x ≈m x.
+    Proof. apply mb_equiv_refl. Qed.
+
+    Let HA0 : mb_member_ext mem.
+    Proof. apply HA. Qed.
+
+    Let HA1 : ψ x0  ∈m ψ d.
+    Proof. apply HA. Qed.
+
+    Let HA2 : mb_transitive mem (ψ d).
+    Proof. apply HA. Qed.
+
+    Let HA3 : forall x, In x (fol_vars B) -> ψ x ∈m ψ d.
+    Proof. apply Σ2_list_in_spec, HA. Qed.
+
+    Let HA5 : fol_sem M2 ψ (Σ_Σ2 ρ µ d B).
+    Proof. apply HA. Qed.
+
+    Let P x := (if mem_dec x (ψ d) then true else false) = true.
+
+    Let HP0 x : P x <-> mem x (ψ d).
+    Proof.
+      unfold P.
+      destruct (mem_dec x (ψ d)); split; try tauto; discriminate.
+    Qed.
+
+    Let X := sig P.
+
+    Let Hx0 : P (ψ x0).
+    Proof. apply HP0; auto. Qed.
+
+    Let memX (x y : X) := proj1_sig x ∈m proj1_sig y.
+
+    Let equivX_spec (x y : X) : mb_equiv memX x y <-> mb_equiv mem (proj1_sig x) (proj1_sig y).
+    Proof.
+      revert x y; intros (x & Hx) (y & Hy); simpl.
+      unfold mb_equiv, memX; simpl; split.
+      2: { intros H []; apply H. }
+      intros H a; split; intros Ha.
+      + assert (H1 : P a).
+        { apply HP0; revert Hx; rewrite HP0; apply HA2; auto. }
+        revert Ha; apply (H (exist _ a H1)).
+      + assert (H1 : P a).
+        { apply HP0; revert Hy; rewrite HP0; apply HA2; auto. }
+        revert Ha; apply (H (exist _ a H1)).
+    Qed.
+
+    Let HP1 : finite_t (sig P).
+    Proof.
+      apply fin_t_finite_t.
+      + intros; apply eq_bool_pirr.
+      + apply finite_t_fin_t_dec; auto.
+        intro; apply bool_dec.
+    Qed.
+
+    Let HA3' : forall n, In n (fol_vars B) -> P (ψ n).
+    Proof. intros n Hn; apply HP0, HA3; auto. Qed.
+
+    Let Rf s (v : vec X (ar_syms Σ s)) (x : X) :=
+      mb_is_tuple_in mem (ψ (ρ s)) (proj1_sig x##vec_map (@proj1_sig _ _) v). 
+
+    Let HA4 s : In s (fol_syms A) -> is_graph_equiv_function (Rf s) (mb_equiv memX).
+    Proof.
+      intros H.
+      simpl in HA; do 4 apply proj2 in HA.
+      apply proj1 in HA.
+      rewrite fol_sem_lconj in HA.
+      specialize (HA (Σ2_is_fun d (ρ s) ⟑ Σ2_is_tot (ar_syms _ s) d (ρ s))).
+      rewrite fol_sem_bin_fix in HA.
+      destruct HA as (F1 & F2).
+      { apply in_map_iff; exists s; auto. }
+      rewrite Σ2_is_fun_spec in F1.
+      rewrite Σ2_is_tot_spec in F2.
+      split.
+      + intros v (x1 & Hx1) (x2 & Hx2) H1 H2.
+        apply equivX_spec; simpl.
+        unfold mem; red in F1.
+        red in H1; simpl in H1.
+        destruct H1 as (p & (w1 & G1 & G2) & G3).
+        destruct H2 as (q & (w2 & G4 & G5) & G6).
+        apply F1 with p q w1; auto.
+        * apply HP0; auto.
+        * apply HP0; auto.
+        * generalize (mb_is_tuple_fun mem_dec HA0 _ _ _ G2 G5).
+          intros; revert G4; apply mb_is_opair_congruence; auto.
+      + intros v.
+        specialize (F2 (vec_map (@proj1_sig _ _) v)).
+        destruct F2 as (x & p & t & G1 & G2 & G3 & G4).
+        * intros p; rew vec; apply HP0, (proj2_sig (vec_pos v p)).
+        * unfold Rf.
+          apply HP0 in G1.
+          exists (exist _ x G1); simpl.
+          exists p; split; simpl; auto.
+          exists t; simpl; auto.
+    Qed.
+
+    Let HA4' s : In s (fol_syms A) 
+             -> { f : vec X (ar_syms _ s) -> X 
+                | forall v x, x = f v
+                          <-> mb_is_tuple_in mem (ψ (ρ s)) (proj1_sig x##vec_map (@proj1_sig _ _) v) }.
+    Proof.
+      intros H.
+      destruct graph_equiv_function_reif with (4 := HA4 _ H)
+        as (f & Hf); auto.
+      + intros; apply mb_is_tuple_in_dec; auto.
+      + intros v y1 y2 ?; unfold Rf.
+        intros (t & (p & H1 & H2) & H3); exists t; split; auto.
+        exists p; split; auto.
+        revert H1; apply mb_is_opair_congruence; auto.
+        apply equivX_spec; auto.
+      + exists f; intros v x.
+        specialize (Hf v x).
+        unfold Rf in Hf.
+        rewrite Hf. 
+        rewrite equivX_spec.
+        split.
+        * intros ->; auto.
+        * generalize x (f v); clear x v Hf.
+          intros (x & Hx) (y & Hy); simpl.
+          rewrite Mmem; intros ->; f_equal.
+          apply eq_bool_pirr.
+    Qed.
+
+    Let fn s := 
+      match in_dec Hs s (fol_syms A) with
+        | left Hs => proj1_sig (HA4' s Hs)
+        | right _ => fun _ => exist _ _ Hx0
+      end.
+ 
+    Let Hfn s : In s (fol_syms A) 
+               -> forall v x, x = fn s v
+                          <-> mb_is_tuple_in mem (ψ (ρ s)) (proj1_sig x##vec_map (@proj1_sig _ _) v).
+    Proof.
+      intros H.
+      unfold fn.
+      destruct (in_dec Hs s (fol_syms A)) as [ C | [] ]; auto.
+      apply (proj2_sig (HA4' s C)).
+    Qed.
+
+    Let M : fo_model Σ (sig P).
+    Proof.
+      exists.
+      + intros s; apply (fn s).
+      + intros r v.
+        exact (mb_is_tuple_in mem (ψ (µ r)) (vec_map (@proj1_sig _ _) v)).
+    Defined.
+
+    Let M_dec : fo_model_dec M.
+    Proof. intros r v; apply mb_is_tuple_in_dec; auto. Qed.
+
+    Let φ n := 
+      match in_dec eq_nat_dec n (fol_vars B) with
+        | left H  => exist _ _ (HA3' _ H)
+        | right _ => exist _ _ Hx0
+      end.
+
+    Let f : X -> Y := @proj1_sig _ _.
+
+    Let g (y : Y) : X.
+    Proof.
+      refine (match mem_dec y (ψ d) with
+        | left  H => exist _ y _
+        | right _ => exist _ _ Hx0
+      end); apply HP0, H.
+    Defined.
+
+    Let symsB : incl (fol_syms B) (fol_syms A).
+    Proof.
+      red; apply Forall_forall.
+      apply fol_syms_subst.
+      + intros; simpl; auto.
+      + apply Forall_forall; auto.
+    Qed.
+
+    Let HB : fol_sem M φ B.
+    Proof.
+      revert HA5.
+      apply Σ_Σ2_sem with (f := f) (g := g) (d := d) (φ := φ) (ψ := ψ) (F := B)
+                               (ρ := ρ) (µ := µ) (MY := M2) (MX := M) (dy := ψ d); auto.
+      + intros (x & Hx); apply HP0; auto.
+      + intros y Hy; apply HP0 in Hy.
+        exists (exist _ y Hy); auto.
+      + intros (x & Hx); unfold g; simpl.
+        destruct (mem_dec x (ψ d)) as [ | [] ].
+        * f_equal; apply eq_bool_pirr.
+        * apply HP0; auto.
+      + intros i Hi; unfold φ.
+        destruct (in_dec eq_nat_dec i (fol_vars B)) as [ | [] ]; auto.
+      + intros s v H.
+        unfold M; simpl; tauto.
+    Qed.
+
+    Local Lemma SAT2_ext_eq_to_SAT : exists X, fo_form_fin_dec_SAT_in A X.
+    Proof.
+      exists (sig P), M, HP1, M_dec, (fun n => φ (n+2+ns+nr)).
+      revert HB; apply fol_sem_subst.
+    Qed.
+
+  End SAT2_SAT.
+
+  Theorem SAT2_SATn : fo_form_fin_dec_SAT Σ_Σ2_enc
+                   -> fo_form_fin_dec_SAT A.
+  Proof.
+    intros (X & M2 & H1 & H2 & psy & H3).
+    assert (He : Σ2_model_ext M2) by apply H3.
+    destruct (Sig2_ext_discr H1 H2 He psy _ H3) 
+      as (Y & M & G1 & G2 & G3 & G4 & G5 & ψ).
+    apply (SAT2_ext_eq_to_SAT G1 G2 ψ G4).
+  Qed.
+
+End Sig_Sig2_encoding.
+
+Check SAT2_SATn.
+
+Section SATn_SAT2.
+
+  Variable n : nat.
+
+  (** This is the hard implication. From a model of A, 
+      build a model of Σn_Σ2_enc A in hereditary finite sets *)
+
+  Section nested.
+
+    Variables (A : fol_form (Σrel n))
+              (X : Type) (Mn : fo_model (Σrel n) X)
+              (X_fin : finite_t X)
+              (X_discr : discrete X)
+              (Mn_dec : fo_model_dec Mn)
+              (φ : nat -> X)
+              (HA : fol_sem Mn φ A).
+
+    Let R := fom_rels Mn tt.
+
+    Local Lemma SATn_to_SAT2 : exists Y, fo_form_fin_dec_SAT_in (@Σn_Σ2_enc n A) Y.
+    Proof.
+      destruct reln_hfs with (R := fom_rels Mn tt)
+        as (Y & H1 & H2 & mem & H3 & l & r & i & s & H4 & H5 & H6 & H7 & H8 & H9 & H10); auto.
+      exists Y, (bin_rel_Σ2 mem), H1, (bin_rel_Σ2_dec _ H3), 
+        (fun n => match n with 
+           | 0 => l
+           | 1 => r
+           | S (S n) => i (φ n)
+         end).
+      unfold Σn_Σ2_enc; msplit 3; auto.
+      + exists (i (φ 0)); simpl; rew fot; simpl; auto.
+      + apply Σ2_list_in_spec.
+        intros n'; simpl.
+        rewrite fol_vars_map, in_map_iff.
+        intros (m & <- & ?); auto.
+      + rewrite <- Σn_Σ2_correct with (Mn := Mn) (R := fun x y => y = i x) 
+            (φ := fun n => match n with 0 => φ 0 | 1 => φ 1 | S (S n) => φ n end); auto.
+        * rewrite fol_sem_subst.
+          revert HA; apply fol_sem_ext.
+          intros; simpl; rew fot; auto.
+        * intros x; exists (i x); split; auto; apply H6.
+        * intros v w E; rewrite H9.
+          apply fol_equiv_ext; f_equal.
+          apply vec_pos_ext; intro; rew vec.
+        * intros n'; rewrite fol_vars_map, in_map_iff.
+          intros (m & <- & Hm); simpl; auto.
+    Qed.
+
+  End nested.
+
+  Theorem SATn_SAT2 A : fo_form_fin_discr_dec_SAT A
+                     -> fo_form_fin_dec_SAT (@Σn_Σ2_enc n A).
+  Proof.
+    intros (X & H1 & Mn & H2 & H4 & psy & H5).
+    apply SATn_to_SAT2 with X Mn psy; auto.
+  Qed.
+
+End SATn_SAT2.
